[isasat] if delayed use proper length for phases
Because we make it possible for phases to be delayed until the next
restart. Therefore we should use the current conflict count, and
not the count when we should have switched

Weidenbach_Book/IsaSAT/IsaSAT_Rephase.thy
@@ -175,8 +175,8 @@ definition current_phase_letter :: \<open>64 word \<Rightarrow> 64 word\<close> 
       else 70)
      \<close>
 
-definition phase_rephase :: \<open>64 word \<Rightarrow> phase_save_heur \<Rightarrow> phase_save_heur nres\<close> where
-\<open>phase_rephase = (\<lambda>b (\<phi>, target_assigned, target, best_assigned, best, end_of_phase, curr_phase,
+definition phase_rephase :: \<open>64 word \<Rightarrow> 64 word \<Rightarrow> phase_save_heur \<Rightarrow> phase_save_heur nres\<close> where
+\<open>phase_rephase = (\<lambda>end_of_phase b (\<phi>, target_assigned, target, best_assigned, best, _, curr_phase,
      length_phase).
   do {
       let target_assigned = 0;
@@ -210,7 +210,7 @@ definition phase_rephase :: \<open>64 word \<Rightarrow> phase_save_heur \<Right
 
 lemma phase_rephase_spec:
   assumes \<open>phase_save_heur_rel \<A> \<phi>\<close>
-  shows \<open>phase_rephase b \<phi> \<le> \<Down>Id (SPEC(phase_save_heur_rel \<A>))\<close>
+  shows \<open>phase_rephase end_of_phase b \<phi> \<le> \<Down>Id (SPEC(phase_save_heur_rel \<A>))\<close>
 proof -
   obtain \<phi>' target_assigned target best_assigned best end_of_phase curr_phase where
     \<phi>: \<open>\<phi> = (\<phi>', target_assigned, target, best_assigned, best, end_of_phase, curr_phase)\<close>
