Weidenbach_Book/IsaSAT/IsaSAT_Rephase_State.thy
@@ -2,24 +2,24 @@ theory IsaSAT_Rephase_State
   imports IsaSAT_Rephase IsaSAT_Setup IsaSAT_Show
 begin
 
-definition rephase_heur_stats :: \<open>64 word \<Rightarrow> restart_heuristics \<Rightarrow> restart_heuristics nres\<close> where
-  \<open>rephase_heur_stats = (\<lambda>b (fast_ema, slow_ema, restart_info, wasted, \<phi>, relu).
+definition rephase_heur_stats :: \<open>64 word \<Rightarrow> 64 word \<Rightarrow> restart_heuristics \<Rightarrow> restart_heuristics nres\<close> where
+  \<open>rephase_heur_stats = (\<lambda>end_of_phase b (fast_ema, slow_ema, restart_info, wasted, \<phi>, relu).
     do {
-      \<phi> \<leftarrow> phase_rephase b \<phi>;
+      \<phi> \<leftarrow> phase_rephase end_of_phase b \<phi>;
       RETURN (fast_ema, slow_ema, restart_info, wasted, \<phi>, relu)
    })\<close>
 
 
-definition rephase_heur :: \<open>64 word \<Rightarrow> isasat_restart_heuristics \<Rightarrow> isasat_restart_heuristics nres\<close> where
-  \<open>rephase_heur = (\<lambda>b heur.
+definition rephase_heur :: \<open>64 word \<Rightarrow> 64 word \<Rightarrow> isasat_restart_heuristics \<Rightarrow> isasat_restart_heuristics nres\<close> where
+  \<open>rephase_heur = (\<lambda>end_of_phase b heur.
   do {
-  \<phi> \<leftarrow> rephase_heur_stats b (get_content heur);
+  \<phi> \<leftarrow> rephase_heur_stats end_of_phase b (get_content heur);
   RETURN (Restart_Heuristics \<phi>)
   })\<close>
 
 
 lemma rephase_heur_spec:
-  \<open>heuristic_rel \<A> heur \<Longrightarrow> rephase_heur b heur \<le>  \<Down>Id (SPEC(heuristic_rel \<A>))\<close>
+  \<open>heuristic_rel \<A> heur \<Longrightarrow> rephase_heur end_of_phase b heur \<le>  \<Down>Id (SPEC(heuristic_rel \<A>))\<close>
   unfolding rephase_heur_def rephase_heur_stats_def
   apply (refine_vcg phase_rephase_spec[THEN order_trans])
   apply (auto simp: heuristic_rel_def heuristic_rel_stats_def)
@@ -27,10 +27,11 @@ lemma rephase_heur_spec:
 
 definition rephase_heur_st :: \<open>isasat \<Rightarrow> isasat nres\<close> where
   \<open>rephase_heur_st = (\<lambda>S. do {
+      let lcount = get_global_conflict_count S;
       let heur = get_heur S;
       let stats = get_stats_heur S;
       let b = current_restart_phase heur;
-      heur \<leftarrow> rephase_heur b heur;
+      heur \<leftarrow> rephase_heur lcount b heur;
       let _ = isasat_print_progress (current_phase_letter (current_rephasing_phase heur))
                   b stats (get_learned_count S);
       RETURN (set_heur_wl_heur heur S)
